

## Derivation

we have

$$a_{ij} = \left[ \sum_{k=1}^n l_{ik} u_{kj} \right]$$

if  $i > j$

$$a_{ij} = \sum_{k=1}^j l_{ik} u_{kj} + l_{ij} u_{jj}$$

$$a_{ij} = \sum_{k=1}^j l_{ik} u_{kj} = \sum_{k=1}^{j-1} l_{ik} u_{kj} + l_{ij} u_{jj}$$

if  $i < j$

$$a_{ij} = \sum_{k=1}^i l_{ik} u_{kj} = \sum_{k=1}^{i-1} l_{ik} u_{kj} + l_{ii} u_{ij}$$

then  $u_{jj} = 1$

$$\Rightarrow l_{ij} = a_{ij} - \sum_{k=1}^{j-1} l_{ik} u_{kj}$$

$$u_{ij} = \frac{1}{l_{ii}} \left( a_{ij} - \sum_{k=1}^{i-1} l_{ik} u_{kj} \right)$$

For Cholesky

$$l_{ij} = \frac{1}{l_{jj}} \left( a_{ij} - \sum_{k=1}^{j-1} l_{ik} l_{kj} \right)$$

$$i < j$$

$$l_{ij} = \frac{1}{l_{ii}} \left( a_{ij} - \sum_{k=1}^{i-1} l_{ik} l_{kj} \right)$$

$$i < j$$

$$l_{ij} = \frac{1}{l_{ii}} \left( a_{ij} - \sum_{k=1}^{i-1} l_{ik} l_{kj} \right)$$

if  $i = j$

$$a_{ii} = \sum_{k=1}^i l_{ik} u_{ii} = \sum_{k=1}^{i-1} l_{ik}^2 + l_{ii}^2$$

$$l_{ii} = \pm \sqrt{a_{ii} - \sum_{k=1}^{i-1} l_{ik}^2}$$